ML_SP_Domain.v
@@ -1,4 +1,7 @@
-(* $Id$ *)
+(***************************************************************************
+* Preservation and Progress for mini-ML with structural polymorphism       *
+* Jacques Garrigue, October 2007                                           *
+***************************************************************************)
 
 Set Implicit Arguments.
 Require Import Lib_FinSet Metatheory List Arith
@@ -97,19 +100,6 @@ Module Delta.
                    (combine l (map typ_bvar (seq 2 (length l))))) ::
              map (fun _ => None) (seq 0 (S (length l))))
     end.
-
-  Lemma closed : forall c, sch_fv (Delta.type c) = {}.
-  Proof.
-    intros.
-    induction c; unfold sch_fv; simpl.
-      rewrite union_empty_l. rewrite* union_empty_l.
-    assert (exists x, x=1). exists 1. auto.
-    destruct H. pattern 1 at -1. rewrite <- H.
-    generalize x.
-    induction l; simpl; intros; rewrite union_empty_l; rewrite* union_empty_l.
-    rewrite union_empty_l. apply IHl.
-  Qed.
-
   Definition matches_lhs l k :=
     trm_app
       (const_app (Const.matches l) (map trm_bvar (seq 1 (length l))))
@@ -152,6 +142,20 @@ Module Delta.
     unfold matches_rhs.
     apply cln_app; apply cln_bvar; omega.
   Qed.
+
+  Lemma closed : forall c, sch_fv (Delta.type c) = {}.
+  Proof.
+    intros.
+    induction c; unfold sch_fv; simpl. unfold kind_fv; simpl.
+      repeat rewrite union_empty_l. auto.
+    assert (exists x, x=1). exists 1. auto.
+    destruct H. pattern 1 at -1. rewrite <- H.
+    generalize x.
+    induction l; simpl; unfold kind_fv in *; simpl in *; intros;
+      repeat rewrite union_empty_l.
+      auto.
+    use (IHl (S x0)); clear IHl. rewrite union_empty_l in H0. auto.
+  Qed.
 End Delta.
 
 Module Sound2 := Mk2(Delta).
@@ -159,7 +163,8 @@ Import Sound2.
 Import JudgInfra.
 Import Judge.
 
-Section For_all2.
+Module SndHyp.
+  Section For_all2.
   Variables (A B:Set) (P:A->B->Prop).
 
   Lemma For_all2_app : forall u1 u2 v1 v2,
@@ -169,19 +174,6 @@ Section For_all2.
     induction u1; intros; destruct* u2; try elim H.
     simpl; intros.
     split*.
-  Qed.
-
-  Lemma For_all2_app' : forall v1 v2 u1 u2,
-    For_all2 P (app u1 v1) (app u2 v2) ->
-    length u1 = length u2 ->
-    For_all2 P u1 u2 /\ For_all2 P v1 v2.
-  Proof.
-    induction u1; intros; destruct* u2; try discriminate.
-      simpl in *. auto.
-    simpl in *.
-    destruct H.
-    inversion H0; clear H0.
-    destruct* (IHu1 u2).
   Qed.
 
   Lemma For_all2_nth : forall d1 d2 n l1 l2,
@@ -208,9 +200,8 @@ Section For_all2.
     apply* For_all2_app.
     simpl. auto.
   Qed.
-End For_all2.
+  End For_all2.
 
-Module SndHyp.
   Lemma fold_arrow_eq : forall T1 TL1 T2 TL2 Us,
     typ_open (fold_right typ_arrow T1 TL1) Us = fold_right typ_arrow T2 TL2 ->
     length TL1 = length TL2 ->
@@ -222,529 +213,24 @@ Module SndHyp.
     destruct* (IHTL1 T2 TL2 Us).
   Qed.
 
-  Lemma kenv_ok_concat_inv : forall K K',
-    kenv_ok (K & K') -> kenv_ok K /\ kenv_ok K'.
+  Lemma fold_app_inv : forall K E t tl T,
+    K ; E |(false,GcLet)|= fold_left trm_app tl t ~: T ->
+    exists TL,
+      K ; E |(false,GcLet)|= t ~: fold_right typ_arrow T TL /\
+      For_all2 (typing (false,GcLet) K E) tl TL.
   Proof.
-    intros; destruct H.
-    destruct (ok_concat_inv _ _ H).
-    split; split*; intros x a B; apply* (H0 x).
-  Qed.
-
-  Lemma kenv_ok_open_fresh : forall K Ks Xs,
-    kenv_ok K ->
-    kenv_ok (kinds_open_vars Ks Xs) -> 
-    fresh (dom K) (length Ks) Xs ->
-    kenv_ok (K & kinds_open_vars Ks Xs).
-  Proof.
-    intros.
-    split*.
-      unfold kinds_open_vars.
-      apply* disjoint_ok.
-      rewrite mkset_dom. apply disjoint_comm.
-      apply* (fresh_disjoint (length Ks)).
-      unfold kinds_open. rewrite map_length.
-      rewrite* (fresh_length _ _ _ H1).
-    intros x a B.
-    binds_cases B.
-      apply* (proj2 H x).
-    apply* (proj2 H0 x).
-  Qed.
-
-  Lemma typing_app_inv : forall K E t1 t2 T,
-    K; E |= trm_app t1 t2 ~: T ->
-    forall E' t' T',
-    (forall K' U,
-      K & K'; E |= t1 ~: typ_arrow U T ->
-      K & K'; E |= t2 ~: U ->
-      K & K'; E' |= t' ~: T') ->
-    K; E' |= t' ~: T'.
-  Proof.
-    introv Typ.
-    gen_eq (trm_app t1 t2) as t0.
-    induction Typ; intros; try discriminate.
-      inversions H. use (H0 (empty(A:=kind)) S).
-    apply* (typing_gc Ks L).
-    intros. apply* H0.
-    intro. rewrite concat_assoc.
-    apply* H2.
-  Qed.
-
-  Lemma trm_fv_open : forall t' t n,
-    trm_fv (trm_open_rec n t' t) << trm_fv t \u trm_fv t'.
-  Proof.
-    induction t; simpl; intros; intros x Hx; auto*.
-    destruct (n0 === n). rewrite* union_empty_l.
-      elim (in_empty Hx).
-    apply* S.union_2.
-    apply* (IHt (S n)).
-    destruct (S.union_1 Hx).
-      destruct* (S.union_1 (IHt1 n x H)); auto with sets.
-      destruct* (S.union_1 (IHt2 (S n) x H)); auto with sets.
-    destruct (S.union_1 Hx).
-      destruct* (S.union_1 (IHt1 n x H)); auto with sets.
-      destruct* (S.union_1 (IHt2 n x H)); auto with sets.
-    elim (in_empty Hx).
-  Qed.
-
-  Lemma typing_strengthen : forall y s t K E E' T,
-    K ; E & y ~ s & E' |= t ~: T ->
-    y \notin trm_fv t ->
-    K ; E & E' |= t ~: T.
-  Proof.
-    introv Typ. gen_eq (E & y ~ s & E') as E0. gen E E'.
-    induction Typ; intros; subst; auto*.
-      binds_cases H1.
-        apply* typing_var.
-        simpl in H4. elim H4. apply* (proj2 (in_singleton x x)).
-        apply* typing_var.
-      apply* typing_abs.
-        intros.
-        rewrite concat_assoc.
-        apply* H1.
-    intro.
-    destruct (S.union_1 (trm_fv_open _ _ _ H4)).
-      elim (H3 H5).
-      use (proj42 (typing_regular (H0 _ H2))).
-      use (ok_remove _ _ _ H6); clear H6.
-      inversions H7.
-      elim H11.
-      rewrite* (proj1 (in_singleton _ _) H5).
-      simpl. auto with sets.
-    apply* typing_let.
-      intros. apply* H0. simpl in H4. auto*.
-      intros. rewrite concat_assoc. apply* H2.
-    intro.
-    destruct (S.union_1 (trm_fv_open _ _ _ H5)).
-      elim H4. simpl. auto with sets.
-      use (proj42 (typing_regular (H1 _ H3))).
-      use (ok_remove _ _ _ H7); clear H7.
-      inversions H8.
-      elim H12; simpl.
-      rewrite (proj1 (in_singleton _ _) H6). auto with sets.
-    simpl in H0.
-    apply* typing_app.
-  Qed.
-
-  Lemma typing_var_inv : forall K E x T,
-    K ; E |= trm_fvar x ~: T ->
-    exists M, binds x M E /\
-      exists Us, T = sch_open M Us /\
-        exists K', kenv_ok (K & K') /\ proper_instance (K & K') M Us.
-  Proof.
-    introv Typ; gen_eq (trm_fvar x) as t.
-    induction Typ; intros; subst; try discriminate.
-      inversions H3. exists M; intuition.
-      exists Us; intuition.
-      exists (empty(A:=kind)). simpl*.
-    pick_freshes (length Ks) Xs.
-    destruct* (H0 Xs) as [M [B [Us [HT [K' [Kok PI]]]]]].
-    exists M; intuition.
-    exists Us; intuition.
-    rewrite concat_assoc in *.
-    exists* (kinds_open_vars Ks Xs & K').
-  Qed.
-
-  Lemma typing_strengthen' : forall K E t T E',
-    K ; E |= t ~: T ->
-    ok E' ->
-    trm_fv t << dom E' ->
-    extends E' E ->
-    K ; E' |= t ~: T.
-  Proof.
-    introv Typ. gen E'.
-    induction Typ; intros.
-    apply* typing_var.
-      simpl in H4.
-      case_eq (get x E'); intros.
-        rewrite (binds_func (H5 x _ H6) H1) in H6. auto.
-      elim (get_none_notin _ H6).
-      apply H4. auto with sets.
-    apply_fresh* typing_abs as y.
-      apply* H1.
-        intros x Hx.
-        use (trm_fv_open _ _ _ Hx).
-        rewrite dom_concat.
-        simpl in *.
-        destruct (S.union_1 H5); auto with sets.
-      intros x M B.
-      binds_cases B.
-        apply* binds_concat_ok.
-        forward~ (H0 y) as Hy.
-      apply* binds_prepend.
-    apply_fresh* (typing_let (M:=M) (L1 \u dom K)) as y.
-      intros.
-      apply* H0.
-      intros x Hx; apply H4.
-      simpl; auto with sets.
-      apply* H2.
-      intros x Hx.
-      simpl in *.
-      destruct (S.union_1 (trm_fv_open _ _ _ Hx)); auto with sets.
-      intros x M' B.
-      binds_cases B.
-        apply* binds_concat_ok.
-        forward~ (H1 y) as Hy.
-      apply* binds_prepend.
-    apply* typing_app.
-      apply* IHTyp1.
-      intros x Hx; apply H0. simpl; auto with sets.
-      apply* IHTyp2.
-      intros x Hx; apply H0. simpl; auto with sets.
-    apply* typing_cst.
-    apply* typing_gc.
-  Qed.
-
-  Lemma trm_open_comm : forall u v t i j,
-    term u -> term v -> i <> j ->
-    {j ~> v}({i ~> u}t) = {i ~> u}({j ~> v}t).
-  Proof.
-    induction t; intros; simpl; auto.
-    destruct (i === n); simpl; destruct* (j === n).
-      elim H1; rewrite* e.
-      simpl. destruct* (i === n). rewrite* <- Infra.trm_open_rec.
-      rewrite* <- Infra.trm_open_rec.
-    simpl. destruct* (i === n).
-    rewrite* IHt.
-    rewrite* IHt1. rewrite* IHt2.
-    rewrite* IHt1. rewrite* IHt2.
-  Qed.
-
-(*
-  Lemma typing_rename : forall K E t1 x T1 T,
-    x \notin (dom E \u trm_fv t1) ->
-    K ; E & x ~ T1 |= t1 ^ x ~: T ->
-    forall y,
-      y \notin (dom E \u trm_fv t1 \u {{x}}) ->
-      K ; E & y ~ T1 |= t1 ^ y ~: T.
-  Proof.
-    intros.
-    replace (E & y ~ T1) with (E & y ~ T1 & nil) by simpl*.
-    replace (t1 ^ y) with (trm_subst x (trm_fvar y) (t1 ^ x)).
-      apply* (typing_trm_subst nil (M:=T1)).
-      rewrite concat_assoc. simpl (x ~ T1 & nil).
-      apply* typing_weaken.
-      destruct (ok_concat_inv _ _ (proj42 (typing_regular H0))).
-      apply* disjoint_ok.
-        simpl; intro.
-        case_eq (S.mem x0 ({{y}} \u dom E)); intros.
-          right; intro.
-          destruct (S.union_1 H5).
-            use (proj1 (in_singleton _ _) H6); subst; clear H5 H6.
-            destruct (S.union_1 (S.mem_2 H4)).
-              use (proj1 (in_singleton _ _) H5); subst; clear H5.
-              elim H1; auto with sets.
-            elim H; auto with sets.
-          elim (in_empty H6).
-        left; intro.
-        rewrite (S.mem_1 H5) in H4. discriminate.
-      exists (dom K \u fv_in kind_fv K \u env_fv E \u typ_fv (sch_type T1)).
-      intros Xs Fr.
-      unfold sch_open_vars, typ_open_vars.
-      fold (sch_open T1 (typ_fvars Xs)).
-      apply* typing_var.
-        split.
-          unfold kinds_open_vars, kinds_open.
-          apply* disjoint_ok. apply* ok_combine_fresh.
-          rewrite mkset_dom.
-          apply disjoint_comm.
-          apply* (fresh_disjoint (sch_arity T1)).
-          rewrite map_length. rewrite <- (fresh_length _ _ _ Fr).
-          reflexivity.
-        (* impossible... *)
-  
-  Lemma typing_abs_inv : forall K E t1 U T,
-    K ; E |= trm_abs t1 ~: typ_arrow U T ->
-    forall x, x \notin (dom E \u trm_fv t1) ->
-      K ; (E & x ~ Sch U nil) |= (t1 ^ x) ~: T.
-  Proof.
-    intros.
-    gen_eq (trm_abs t1) as t; gen_eq (typ_arrow U T) as T0; gen x.
-    induction H; intros; try discriminate.
-      inversions H3; inversions H4; clear H3 H4.
-      destruct (var_fresh (dom E \u trm_fv t1 \u L)) as [y Fr].
-      exists* L.
-    subst.
-    pick_freshes (length Ks) Xs.
-    destruct* (H0 Xs) as [L' R].
-    exists L'.
-    intros; apply (typing_gc Ks L).
-    intros.
-    destruct* (H0 Xs0) as [L'' R']; clear H0 R Fr.
-    apply* R'.
-
-  Lemma fv_in_concat : forall (A : Set) (fv : A -> vars) E F,
-    fv_in fv (E & F) = fv_in fv F \u fv_in fv E.
-  Proof.
-    induction F; simpl.
-      rewrite* union_empty_l.
-    destruct a. rewrite IHF. rewrite* union_assoc.
-  Qed.
-
-  Lemma fv_in_combine : forall Xs Ks,
-    length Xs = length Ks ->
-    fv_in kind_fv (combine Xs Ks) = kind_fv_list Ks.
-  Proof.
-    induction Xs; intros; destruct Ks; try discriminate; simpl in *.
-      auto.
-    rewrite* IHXs.
-  Qed.
-
-  Lemma notin_typ_open : forall x T Us,
-    x \notin typ_fv T -> x \notin typ_fv_list Us ->
-    x \notin typ_fv (typ_open T Us).
-  Proof.
-    induction T; simpl; intros; auto.
-      gen n; induction Us; simpl in *; intros; destruct* n.
-    apply* notin_union_l.
-  Qed.
-
-  Lemma notin_kinds_open : forall x Ks Us,
-    x \notin kind_fv_list Ks ->
-    x \notin typ_fv_list Us ->
-    x \notin kind_fv_list (kinds_open Ks Us).
-  Proof.
-    induction Ks; simpl; intros.
-      auto.
-    apply* notin_union_l.
-    unfold kind_open, kind_fv in *.
-    destruct a as [[kc kr]|]; simpl in *.
-      induction kr; simpl. auto.
-      destruct a; simpl in *.
-      apply* notin_union_l.
-      apply* notin_typ_open.
-      auto*.
-  Qed.
-
-  Lemma notin_dec : forall x E, x \in E \/ x \notin E.
-    intros.
-    case_eq (S.mem x E); intros.
-      use (S.mem_2 H).
-    right; intro.
-    rewrite (S.mem_1 H0) in H. discriminate.
-  Qed.
-
-  Lemma typ_fv_list_fvars : forall Xs,
-    typ_fv_list (typ_fvars Xs) = mkset Xs.
-  Proof.
-    induction Xs; simpl; auto.
-    rewrite* IHXs.
-  Qed.
-
-  Lemma disjoint_fresh : forall n Xs L' L,
-    fresh L n Xs ->
-    disjoint (mkset Xs) L' ->
-    fresh L' n Xs.
-  Proof.
-    induction n; intros; destruct Xs; use (fresh_length _ _ _ H);
-      try discriminate.
-    simpl in *.
-    split. elim (H0 v); intro; auto. elim H2; auto with sets.
-    apply* IHn.
-    intro.
-    destruct (x == v). subst.
-      elim (fresh_disjoint _ _ _ (proj2 H) v); intro; auto.
-      elim (H0 v); intro; auto.
-    elim (H0 x); intro; auto.
-  Qed.
-
-  Lemma typing_gc_rename : forall Xs Ks K E t T L,
-    L = dom K \u fv_in kind_fv K \u kind_fv_list Ks \u env_fv E \u typ_fv T ->
-    fresh L (length Ks) Xs ->
-    K & kinds_open_vars Ks Xs; E |= t ~: T ->
-    forall Xs',
-      fresh (L \u mkset Xs) (length Ks) Xs' ->
-      K & kinds_open_vars Ks Xs'; E |= t ~: T.
-  Proof.
-    intros.
-    rewrite <- (typ_subst_fresh (combine Xs (typ_fvars Xs')) T).
-    assert (disjoint (mkset Xs) (mkset Xs')).
-      intro.
-      destruct (notin_dec x (mkset Xs')).
-        left; intro. destruct (fresh_union_r _ _ _ _ H2).
-        use (fresh_disjoint _ _ _ H6 x).
-      auto.
-    apply* typing_typ_substs.
-      use (fresh_disjoint _ _ _ H0). rewrite H in H4.
-      rewrite mkset_dom.
-      intro x; destruct (H4 x). left*.
-      elim (H3 x); intro; auto.
-      right.
-      rewrite fv_in_concat. rewrite dom_concat.
-      repeat apply* notin_union_l.
-        unfold kinds_open_vars.
-        rewrite fv_in_combine.
-        apply* notin_kinds_open.
-        rewrite* typ_fv_list_fvars.
-        unfold kinds_open; autorewrite with list.
-        rewrite* (fresh_length _ _ _ H2).
-      unfold kinds_open_vars, kinds_open.
-      rewrite* mkset_dom. rewrite map_length. rewrite* (fresh_length _ _ _ H2).
-      unfold typ_fvars; rewrite map_length. rewrite <- (fresh_length _ _ _ H2).
-      rewrite* (fresh_length _ _ _ H0).
-      clear; gen Xs; induction Xs'; destruct Xs; simpl; intro; intros;
-        try elim (binds_empty H).
-        unfold binds in H; simpl in H.
-        destruct (x == v). inversion* H.
-        apply* (IHXs' Xs x).
-      apply well_subst_open_vars.
-      rewrite fv_in_concat.
-      apply* fresh_union_l.
-      apply* disjoint_fresh.
-      intro.
-      destruct (notin_dec x (mkset Xs)).
-      elim (H3 x); intro; auto.
-      right. unfold kinds_open_vars.
-      rewrite fv_in_combine.
-      apply* notin_kinds_open.
-*)
-
-  Lemma typing_abs_inv0 : forall K E t1 U T,
-    K ; E |= trm_abs t1 ~: typ_arrow U T ->
-    exists L, exists K',
-    forall x, x \notin L ->
-      K & K'; (E & x ~ Sch U nil) |= (t1 ^ x) ~: T.
-  Proof.
-    intros.
-    gen_eq (trm_abs t1) as t; gen_eq (typ_arrow U T) as T0.
-    induction H; intros; try discriminate.
-     exists L. exists (empty(A:=kind)).
-     inversions H2; inversions H3. simpl*.
-    pick_freshes (length Ks) Xs.
-    destruct* (H0 Xs) as [L' [K' R]]; clear H0.
-    exists L'; exists (kinds_open_vars Ks Xs & K').
-    rewrite* <- concat_assoc.
-  Qed.
-
-  Lemma typing_let_inv0 : forall K E t1 t2 T,
-    K ; E |= trm_let t1 t2 ~: T ->
-    exists M, exists K',
-      (exists L1, forall Xs, fresh L1 (sch_arity M) Xs ->
-        K & K' & kinds_open_vars (sch_kinds M) Xs; E |= t1 ~: (M ^ Xs)) /\
-      (exists L2, forall x, x \notin L2 ->
-        K & K' ; (E & x ~ M) |= (t2 ^ x) ~: T).
-  Proof.
-    intros.
-    gen_eq (trm_let t1 t2) as t.
-    induction H; intros; try discriminate.
-     exists M. exists (empty(A:=kind)).
-     inversions H3. simpl*.
-    subst.
-    pick_freshes (length Ks) Xs.
-    destruct* (H0 Xs) as [M [K' R]]; clear H0.
-    exists M; exists (kinds_open_vars Ks Xs & K').
-    repeat rewrite* <- concat_assoc.
-  Qed.
-
-  Lemma binds_dom : forall (A:Set) x (a:A) E,
-    binds x a E -> x \in dom E.
-  Proof.
-    induction E; intros.
-      discriminate.
-    destruct a0.
-    unfold binds in H. simpl in H.
-    simpl. destruct (x == v); auto with sets.
-    rewrite e; auto with sets.
-  Qed.
-
-  Lemma trm_fv_open2 : forall u t i,
-    trm_fv t << trm_fv ({i ~> u}t).
-  Proof.
-    induction t; intros; intros y Hy; simpl; auto with sets.
-    elim (in_empty Hy).
-    apply* IHt.
-    simpl in Hy; unfold S.Subset in *; destruct (S.union_1 Hy); auto with sets.
-    simpl in Hy; unfold S.Subset in *; destruct (S.union_1 Hy); auto with sets.
-  Qed.
-
-  Lemma typing_fv : forall K E t T,
-    K ; E |= t ~: T -> trm_fv t << dom E.
-  Proof.
-    induction 1; simpl; intros y Hy.
-    rewrite (proj1 (in_singleton _ _) Hy). apply* binds_dom.
-    pick_fresh x.
-    forward~ (H1 x) as Hx.
-    simpl in Hx.
-    assert (y \in {{x}} \u dom E).
-      apply Hx. unfold trm_open; apply* trm_fv_open2.
-    destruct* (S.union_1 H2).
-    elim Fr. rewrite (proj1 (in_singleton _ _) H3).
-    repeat (apply S.union_2; try (apply* S.union_3; fail)).
-    pick_fresh x.
-    pick_freshes (sch_arity M) Xs.
-    forward~ (H0 Xs) as Ht1; clear H0.
-    forward~ (H2 x) as Ht2; clear H2.
-    destruct (S.union_1 Hy).
-      apply* Ht1.
-    simpl in Ht2.
-    assert (y \in {{x}} \u dom E).
-      apply Ht2. unfold trm_open; apply* trm_fv_open2.
-    destruct* (S.union_1 H2).
-    elim Fr. rewrite (proj1 (in_singleton _ _) H3).
-    repeat (apply S.union_2; try (apply* S.union_3; fail)).
-    destruct (S.union_1 Hy). apply* IHtyping1. apply* IHtyping2.
-    elim (in_empty Hy).
-    pick_freshes (length Ks) Xs.
-    apply* (H0 Xs).
-  Qed.    
-
-  Lemma typing_var_inv' : forall K E x T t E',
-    K; E |= trm_fvar x ~: T ->
-    (forall K' M Us,
-      kenv_ok (K & K') ->
-      binds x M E ->
-      proper_instance (K & K') M Us ->
-      K & K'; E' |= t ~: sch_open M Us) ->
-    K; E' |= t ~: T.
-  Proof.
-    introv Typ.
-    gen_eq (trm_fvar x) as t0. gen E'.
-    induction Typ; intros; try discriminate.
-      inversions H3. use (H4 (empty(A:=kind)) M).
-    apply* (typing_gc Ks L).
-    intros. apply* H0.
-    intro. rewrite concat_assoc.
-    apply* H2.
-  Qed.
-
-  Lemma typing_abs_inv : forall K E t1 U T,
-    K ; E |= trm_abs t1 ~: typ_arrow U T ->
-    (forall x, t1 ^ x = t1) ->
-    K ; E |= t1 ~: T.
-  Proof.
-    introv Typ; gen_eq (trm_abs t1) as t; gen_eq (typ_arrow U T) as T0.
-    induction Typ; intros; subst; try discriminate.
-      inversions H2; inversions H3; clear H2 H3.
-      destruct (var_fresh (L \u trm_fv t1)) as [x Hx].
-      replace E with (E & empty) by simpl*.
-      apply* typing_strengthen.
-        simpl; simpl in H0. rewrite* <- (H4 x).
-        auto*.
-    apply* typing_gc.
-  Qed.
-
-  Lemma fold_app_inv : forall E t tl K T,
-    K ; E |= fold_left trm_app tl t ~: T ->
-    forall E' t' T',
-    (forall K' TL,
-      K & K'; E |= t ~: fold_right typ_arrow T TL ->
-      For_all2 (typing (K & K') E) tl TL ->
-      K & K'; E' |= t' ~: T') ->
-    K ; E' |= t' ~: T'.
-  Proof.
-    induction tl using rev_ind; simpl; intros.
-      use (H0 empty nil).
+    intros K E t tl.
+    rewrite <- (rev_involutive tl).
+    induction (rev tl); clear tl; simpl; intros.
+      exists (nil(A:=typ)). auto.
     rewrite fold_left_app in *; simpl in *.
-    apply* (typing_app_inv H).
-    intros.
-    apply* IHtl; clear IHtl.
-    intros.
-    rewrite* concat_assoc.
-    apply* (H0 (K' & K'0) (TL ++ U :: nil)); clear H0.
-      rewrite fold_right_app; simpl.
-      rewrite* <- concat_assoc.
-      rewrite* <- concat_assoc.
-    apply* For_all2_app.
-    split*. apply* typing_weaken_kinds'. simpl*.
+    inversions H.
+    destruct (IHl (typ_arrow S T) H4).
+    exists (x ++ S :: nil).
+    rewrite fold_right_app; simpl.
+    split*. apply* For_all2_app.
+    simpl. split*.
+    discriminate.
   Qed.
 
   Lemma map_nth : forall (A B:Set) d1 d2 (f:A->B) k l,
@@ -774,58 +260,12 @@ Module SndHyp.
 
   Hint Rewrite combine_length combine_nth : list.
 
-  Lemma For_all2_imp : forall (A B:Set) (P P' : A -> B -> Prop) l1 l2,
-    For_all2 P l1 l2 ->
-    (forall x y, In (x,y) (combine l1 l2) -> P x y -> P' x y) ->
-    For_all2 P' l1 l2.
-  Proof.
-    induction l1; destruct l2; simpl; intros; auto.
-    split*.
-  Qed.
-
-  Lemma typing_cst_inv' : forall K E c T,
-    K; E |= trm_cst c ~: T ->
-    forall E' t T',
-    (forall K' Us,
-      kenv_ok (K & K') ->
-      proper_instance (K & K') (Delta.type c) Us ->
-      T = sch_open (Delta.type c) Us ->
-      K & K'; E' |= t ~: T') ->
-    K; E' |= t ~: T'.
-  Proof.
-    introv Typ.
-    gen_eq (trm_cst c) as t0.
-    induction Typ; intros; try discriminate.
-      inversions H2. use (H3 (empty(A:=kind)) Us).
-    apply* (typing_gc Ks L).
-    intros. apply* H0.
-    intro. rewrite concat_assoc.
-    apply* H2.
-  Qed.
-
-  Lemma typing_cst_inv : forall K E c T,
-    K; E |= trm_cst c ~: T ->
-    exists K', exists Us,
-      kenv_ok (K & K') /\
-      proper_instance (K & K') (Delta.type c) Us /\
-      T = sch_open (Delta.type c) Us.
-  Proof.
-    introv Typ; gen_eq (trm_cst c) as t.
-    induction Typ; intros; try discriminate.
-      inversions H2. exists (empty(A:=kind)); exists* Us.
-    subst.
-    pick_freshes (length Ks) Xs.
-    destruct* (H0 Xs) as [K' R]; clear H0.
-    exists (kinds_open_vars Ks Xs & K'). rewrite* <- concat_assoc.
-  Qed.
-
-(*
   Lemma get_kind_for_matches : forall k l t K E Us,
     k < length l ->
     proper_instance K (Delta.type (Const.matches l)) Us ->
-    K ; E |= trm_app (trm_cst (Const.tag (nth k l var_default)))
+    K; E |(false,GcLet)|= trm_app (trm_cst (Const.tag (nth k l var_default)))
                     t ~: nth 0 Us typ_def ->
-    K ; E |= t ~: nth (S (S k)) Us typ_def.
+    K; E |(false,GcLet)|= t ~: nth (S (S k)) Us typ_def.
   Proof.
     introv Hk PI Typ.
     destruct PI as [[Arity _] [_ WK]].
@@ -837,30 +277,26 @@ Module SndHyp.
     destruct WK as [WK _].
     inversions WK. clear WK.
     destruct H2 as [_ HE]. simpl in *.
-    destruct (typing_app_inv Typ) as [U [K' [Typ1 Typ2]]]. clear Typ.
-    destruct (typing_cst_inv Typ1) as [Us' [K'' [WK [Eq Kok]]]].
-    destruct WK as [_ [_ WK']].
-    destruct* Us'. discriminate.
+    inversions Typ. clear Typ.
+    inversions H4. clear H4 H8.
+    destruct H9 as [_ [_ WK']].
+    destruct* Us0. simpl in H2. discriminate.
     simpl in WK'. destruct WK' as [_ WK].
-    destruct* Us'.
-    destruct* Us'.
+    destruct* Us0.
+    destruct* Us0.
     destruct WK as [WK _].
     inversions WK. clear WK; simpl in *.
-    unfold sch_open in Eq. simpl in Eq.
-    inversions Eq; clear Eq.
-    use (binds_concat_ok K' H0 (proj1 (proj1 (typing_regular Typ2)))).
-    use (binds_concat_ok K'' H (proj1 Kok)).
-    use (binds_func H2 H1). inversion H4; clear H H1 H4; subst k'0.
-    simpl in H3; destruct H3.
-    use (proj2 Kok x0 (Some k') H2). simpl in H3.
-    exists K'.
-    rewrite (proj2 (proj2 H3) (nth k l var_default) t0 (nth k Us typ_def))
-      in Typ2; auto.
+    inversions H2; clear H2.
+    use (binds_func H0 H1). inversion H; clear H H1; subst k'0.
+    simpl in H4; destruct H4.
+    use (proj2 H7 x (Some k') H0). simpl in H2.
+    rewrite (proj2 (proj2 H2) (nth k l var_default) t0 (nth k Us typ_def))
+      in H6; clear H2; auto.
       unfold Cstr.unique.
       destruct H as [Hlow _]. simpl in Hlow.
       apply* Hlow.
     apply HE.
-    clear HE t0 Typ1 Typ2 H H1.
+    clear HE t0 H6 H7 H H1.
     rewrite* <- combine_nth.
     apply* nth_In_eq.
         rewrite combine_length.
@@ -874,155 +310,50 @@ Module SndHyp.
         rewrite* seq_nth.
       rewrite* seq_length.
     rewrite* min_l.
-  Qed.
-*)
-
-  Lemma cut_list : forall (A:Set) k (l:list A),
-    k < length l ->
-    exists l1, exists a, exists l2, l = l1 ++ a :: l2 /\ length l1 = k.
-  Proof.
-    induction k; intros.
-      destruct l. elim (lt_n_O _ H).
-      exists (nil(A:=A)). exists a. exists* l.
-    destruct l. elim (lt_n_O _ H).
-    destruct* (IHk l) as [l1 [b [l2 [E1 E2]]]].
-      apply (lt_S_n _ _ H).
-    exists (a::l1). exists b. exists* l2.
-    simpl; rewrite E1; rewrite* E2.
-  Qed.
-
-  Lemma seq_app : forall n m k,
-    seq k (m + n) = seq k m ++ seq (m+k) n.
-  Proof.
-    induction m; simpl; intros. auto.
-    rewrite IHm. rewrite <- plus_Snm_nSm. simpl*.
-  Qed.
-
-  Lemma app_nth3 : forall (A:Set) (d:A) l1 a l2,
-    nth (length l1) (l1 ++ a :: l2) d = a.
-  Proof.
-    intros. rewrite* app_nth2. rewrite <- minus_n_n. simpl*.
-  Qed.
-
-  Lemma combine_app : forall (A B:Set) (u2:list A) (v2:list B) u1 v1,
-    length u1 = length v1 ->
-    combine (u1 ++ u2) (v1 ++ v2) = combine u1 v1 ++ combine u2 v2.
-  Proof.
-    induction u1; destruct v1; simpl; intros; try discriminate.
-      auto.
-    inversion H; rewrite* IHu1.
+    discriminate.
+    discriminate.
   Qed.
 
   Lemma delta_typed : forall n t1 t2 tl K E T,
     Delta.rule n t1 t2 ->
     list_for_n term n tl ->
-    K ; E |= trm_inst t1 tl ~: T ->
-    K ; E |= trm_inst t2 tl ~: T.
+    K ; E |(false,GcLet)|= trm_inst t1 tl ~: T ->
+    K ; E |(true,GcAny)|= trm_inst t2 tl ~: T.
   Proof.
     intros.
+    apply (@typing_gc_any (false,GcLet)).
+    clear H0.
     destruct H as [l [k [HN [HK [T1 T2]]]]].
     subst.
-    unfold Delta.matches_lhs, trm_inst in H1. simpl in H1.
-    rewrite trm_inst_app in H1.
-    apply* typing_app_inv; clear H1.
-    intros.
-    unfold const_app in H.
-    apply* fold_app_inv; clear H.
-    intros.
-    unfold Delta.matches_rhs, trm_inst.
-    destruct tl.
-      destruct H0; discriminate.
-    simpl in *.
-    rewrite <- seq_shift in H2.
-    repeat rewrite map_map in H2.
-    simpl in H2.
-    destruct* (cut_list _ HK) as [l1 [v [l2 [El El']]]]. subst l.
-    destruct* (cut_list tl (k:=k)) as [tl1 [f [tl2 [Etl Etl']]]].
-      clear -HK H0.
-      destruct H0. simpl in H; inversion* H.
-    destruct* (cut_list TL (k:=k)) as [TL1 [V [TL2 [ETL ETL']]]].
-      rewrite* <- (For_all2_length _ _ _ H2).
-      rewrite map_length. rewrite* seq_length.
-    rewrite <- El' in H1. rewrite app_nth3 in H1.
-    rewrite Etl. rewrite <- Etl'. rewrite app_nth3.
-    subst; simpl in *.
-    apply* (typing_cst_inv' H); clear H.
-    intros.
-    unfold sch_open, sch_arity in H4; simpl in H4.
-    destruct (fold_arrow_eq _ _ _ _ _ (sym_equal H4)); clear H4.
-      rewrite map_length; rewrite seq_length.
-      rewrite <- (For_all2_length _ _ _ H2).
+    inversions H1; clear H1.
+    rewrite trm_inst_app in H4.
+    unfold const_app in H4.
+    destruct (fold_app_inv _ _ H4) as [TL [Typ0 TypA]]; clear H4.
+    unfold trm_inst; simpl.
+    inversions Typ0. clear Typ0 H1 H4.
+    unfold sch_open in H0. simpl in H0.
+    destruct (fold_arrow_eq _ _ _ _ _ H0); clear H0.
+      generalize (For_all2_length _ _ _ TypA).
       autorewrite with list. auto.
-    unfold sch_open, sch_arity in H5; simpl in H5.
-    inversions H5; clear H5.
-    use (proj1 (proj1 H3)).
-    unfold sch_arity in H4; simpl in H4.
-    do 2 (destruct Us; try discriminate).
-    rewrite map_length in H4; rewrite seq_length in H4. simpl in H4.
-    inversions H4; clear H4.
-    repeat rewrite <- seq_shift in H6. repeat rewrite map_map in H6.
-    rewrite app_length in H6. rewrite seq_app in H6.
-    rewrite map_app in H6.
-    destruct (For_all2_app' _ _ _ _ _ H6) as [_ HA]; clear H6.
-      ssimpl_list. symmetry. trivial.
-    simpl in HA; destruct HA as [Hv _].
-    simpl.
-    use (proj1 (proj1 H3)).
-    unfold sch_arity in H4; simpl in H4.
-    autorewrite with list in H4.
-    inversion H4; clear H4.
-    destruct (cut_list (k:=length l1) Us) as [Us1 [U [Us2 [EUs EUs']]]].
-      omega.
-    rewrite EUs in Hv. rewrite plus_0_r in Hv.
-    rewrite <- EUs' in Hv; rewrite app_nth3 in Hv.
-    simpl in H1.
-    rewrite app_length in H2. rewrite seq_app in H2. rewrite map_app in H2.
-    destruct (For_all2_app' _ _ _ _ _ H2) as [_ HA]; clear H2.
-      ssimpl_list. symmetry. trivial.
-    simpl in HA; destruct HA as [Hf _].
-    rewrite <- Etl' in Hf. rewrite plus_0_r in Hf. rewrite app_nth3 in Hf.
-    subst.
-    apply* typing_app. apply* typing_weaken_kinds'.
-    rewrite concat_assoc in H.
-    use (typing_weaken_kinds' _ H H1); clear H1.
-    rewrite <- concat_assoc in H2.
-    apply* (typing_app_inv H2); clear H2.
-    intros.
-    apply* (typing_cst_inv' H1); clear H1.
-    intros.
-    unfold sch_open, sch_arity in H5; simpl in H5.
-    inversions H5; clear H5.
-    use (proj1 (proj1 H4)).
-    unfold sch_arity in H5; simpl in H5.
-    do 3 (destruct Us; try discriminate). clear H5.
-    simpl in H2.
-    use (proj2 (proj2 H3)). simpl in H5.
-    use (proj2 (proj2 H4)). simpl in H8.
-    use (proj1 (proj2 H8)); clear H8.
-    use (proj1 H5); clear H5.
-    inversions H9; clear H9.
-    inversions H8; clear H8.
-    use (binds_concat_ok (K'2 & K'3) H13).
-    rewrite <- concat_assoc in H5.
-    use (binds_func (H5 (proj1 H1)) H10); clear H5 H13.
-    inversions H8; clear H8.
-    use (proj2 H1 _ _ H10). simpl in H5.
-    assert (Cstr.unique (kind_cstr k') v).
-      destruct H12 as [[Hlow _] _]. simpl in Hlow.
-      apply (Hlow v). auto with sets.
-    rewrite* (proj2 (proj2 H5) v U t0).
-      apply* typing_weaken_kinds'.
-      apply* (proj2 H14).
-      clear -EUs'.
-      simpl.
-      rewrite app_length; rewrite seq_app; repeat rewrite map_app. 
-      rewrite combine_app.
-      rewrite map_app.
-      apply in_or_app. right.
-      simpl. left.
-      rewrite plus_comm. simpl. rewrite <- EUs'. rewrite* app_nth3.
-      ssimpl_list. auto.
-    apply* (proj2 H12 (v, t0)).
+    generalize (For_all2_nth _ trm_def typ_def _ TL TypA (n:=k)); clear TypA.
+    autorewrite with list; intro TypA.
+    generalize (For_all2_nth _ typ_def typ_def _ TL H1 (n:=k)); clear H1.
+    autorewrite with list; intro EQ.
+    rewrite <- EQ in TypA; auto; clear EQ TL.
+    rewrite (map_nth trm_def trm_def) in TypA.
+     rewrite (map_nth trm_def 0) in TypA.
+      rewrite seq_nth in TypA; auto.
+      rewrite (map_nth typ_def 0) in TypA.
+       rewrite seq_nth in TypA; auto.
+       simpl in TypA, H.
+       inversions H; clear H.
+       apply* typing_app.
+       apply* get_kind_for_matches.
+      rewrite* seq_length.
+     rewrite* seq_length.
+    autorewrite with list; auto.
+    discriminate.
+    discriminate.
   Qed.
 
   Lemma cons_append : forall (A:Set) (a:A) l, a :: l = (a :: nil) ++ l.
@@ -1058,61 +389,50 @@ Module SndHyp.
   Qed.
 
   Lemma value_is_tag : forall K v n T,
-    K; empty |= v ~: T ->
+    K; empty |(false,GcLet)|= v ~: T ->
     valu n v ->
     typ_arity T <= n ->
     exists l, exists tl, v = const_app (Const.tag l) tl.
   Proof.
-    introv Typ; gen n.
-    induction Typ; introv Hv TA; try (inversions Hv; fail).
-    inversions Hv.
-    elim (le_Sn_O _ TA).
-    inversions Hv.
-    clear IHTyp2.
-      destruct* (IHTyp1 (Datatypes.S n) H2) as [l [tl EQ]].
+    induction v; introv Typv Hv TA; inversions Hv; inversions Typv;
+      try discriminate.
+      simpl in TA. elim (le_Sn_O _ TA).
+      clear IHv2.
+      destruct* (IHv1 (Datatypes.S n) _ H5) as [l [tl EQ]].
         simpl. apply* le_n_S.
-      exists l. exists (tl ++ t2 :: nil).
+      exists l. exists (tl ++ v2 :: nil).
       rewrite EQ.
       unfold const_app; rewrite fold_left_app. auto.
     destruct c.
       exists v. exists (nil (A:=trm)). auto.
-    inversions Hv.
     elim (le_not_lt _ _ TA). clear.
     unfold sch_open; simpl.
     rewrite fold_arrow_open.
     rewrite typ_arity_fold_arrow.
     autorewrite with list.
     simpl. omega.
-    pick_freshes (length Ks) Xs.
-    apply* (H0 Xs).
   Qed.
 
   Lemma tag_is_const : forall v vl K T TL,
     S (Const.arity (Const.tag v)) = length vl ->
-    K; empty |= trm_cst (Const.tag v) ~: fold_right typ_arrow T TL ->
-    For_all2 (typing K empty) vl TL -> False.
+    K; empty |(false,GcLet)|= trm_cst (Const.tag v) ~:
+      fold_right typ_arrow T TL ->
+    For_all2 (typing (false,GcLet) K empty) vl TL -> False.
   Proof.
     introv Hv TypC TypA.
-    gen_eq (trm_cst (Const.tag v)) as t.
-    gen_eq (fold_right typ_arrow T TL) as T0.
-    induction TypC; intros; subst; try discriminate.
-      inversions H3; clear H3.
-      do 3 (destruct vl; try discriminate).
-      destruct TL; destruct* TypA.
-      destruct TL; destruct* H4.
-      destruct TL; destruct* H5.
-      unfold sch_open in H2; simpl in H2.
-      inversions H2; clear H2.
-      destruct H1 as [_ [_ WK]]. simpl in WK.
-      do 3 destruct* Us.
-      destruct WK as [_ [WK _]].
-      inversions WK.
-      discriminate.
-    pick_freshes (length Ks) Xs.
-    forward~ (H Xs) as Typ.
-    apply* (H0 Xs); clear H0 H.
-    apply* For_all2_imp.
-    intros. apply* typing_weaken_kinds'. apply (proj1 (typing_regular Typ)).
+    inversions TypC; try discriminate. clear TypC H4.
+    destruct* vl; try destruct* vl; try destruct* vl; try discriminate.
+    destruct TL; destruct* TypA.
+    destruct TL; destruct* H2.
+    destruct TL; destruct* H3.
+    unfold sch_open in H0.
+    simpl in H0.
+    inversions H0. clear H0.
+    destruct H5 as [_ [_ WK]]. simpl in WK.
+    destruct* Us. destruct* Us. destruct* Us.
+    destruct WK as [_ [WK _]].
+    inversions WK.
+    discriminate.
   Qed.
 
   Lemma mkset_in : forall x Xs,
@@ -1182,110 +502,86 @@ Module SndHyp.
     elim (le_Sn_O _ H0).
   Qed.
 
-  Lemma fold_app_inv' : forall E t tl K T,
-    K ; E |= fold_left trm_app tl t ~: T ->
-    exists K', exists TL,
-      K & K'; E |= t ~: fold_right typ_arrow T TL /\
-      For_all2 (typing (K & K') E) tl TL.
-  Proof.
-    induction tl using rev_ind; simpl; intros.
-      exists (empty(A:=kind)). exists (nil(A:=typ)). simpl*.
-    rewrite fold_left_app in *. simpl in *.
-    gen_eq (trm_app (fold_left trm_app tl t) x) as t0.
-    induction H; intros; subst; try discriminate.
-      inversions H1; clear H1.
-      destruct (IHtl _ _ H) as [K' [TL [Typ FA]]]; clear IHtl.
-      exists K'; exists (TL ++ S :: nil).
-      rewrite fold_right_app. simpl.
-      split*.
-      apply* For_all2_app. simpl; split*.
-      apply* typing_weaken_kinds'.
-    pick_freshes (length Ks) Xs.
-    destruct* (H0 Xs) as [K' R]; clear H0.
-    exists* (kinds_open_vars Ks Xs & K'). rewrite* <- concat_assoc.
-  Qed.
-
   Lemma typing_tag_inv : forall K l tl x,
-    K; empty |= const_app (Const.tag l) tl ~: typ_fvar x ->
-    exists t, exists T, exists k, exists K',
-      tl = t :: nil /\  K & K'; empty |= t ~: T /\
-      binds x (Some k) (K & K') /\
-      entails k (Kind (Cstr.C {{l}} None) ((l, T) :: nil)).
+    K; empty |(false,GcLet)|= const_app (Const.tag l) tl ~: typ_fvar x ->
+    exists t, exists T, exists k,
+      tl = t :: nil /\  K; empty |(false,GcLet)|= t ~: T /\ binds x (Some k) K
+      /\ entails k (Kind (Cstr.C {{l}} None) ((l, T) :: nil)).
   Proof.
     introv Typv.
-    destruct* (fold_app_inv' _ _ Typv) as [K' [TL [Typ FA]]].
-    destruct* (typing_cst_inv Typ) as [K'' [Us [Kok [[_ [_ WK]] E]]]].
-    unfold sch_open in E; simpl in E.
+    unfold const_app in Typv.
+    destruct* (fold_app_inv _ _ Typv) as [TL [Typc Typa]]; clear Typv.
+    inversions Typc; try discriminate. clear Typc H1 H4.
+    destruct H5 as [_ [_ WK]].
+    unfold sch_open in H0; simpl in H0.
     destruct TL as [|T TL]. discriminate.
-    simpl in E; inversions E; clear E.
-    destruct tl. elim FA.
-    simpl in WK. do 3 destruct* Us.
-    simpl in *.
-    exists t. exists t0.
-    destruct WK as [_ [Ht1 _]].
-    inversions Ht1; clear Ht1.
-    exists k'; exists (K' & K''); rewrite <- concat_assoc.
+    destruct tl. elim Typa.
+    exists t. exists T.
+    simpl in H0; inversions H0; clear H0.
+    simpl in WK.
+    destruct* Us. destruct* Us. destruct* Us.
+    destruct WK as [_ [WK _]]. simpl in WK.
+    inversions WK; clear WK.
+    exists k'.
     destruct TL; try discriminate.
-    destruct FA.
-    destruct tl; try (elim H1).
-    simpl in H4; inversions H4; clear H4.
+    simpl in H2; inversion H2; subst x0; clear H2.
+    simpl in Typa.
+    destruct Typa.
+    destruct tl; try elim H1.
     intuition.
-    apply* typing_weaken_kinds'.
   Qed.
 
   Lemma const_arity_ok0 : forall c vl K T,
     S(Const.arity c) = length vl ->
-    K ; empty |= const_app c vl ~: T ->
+    K ; empty |(false,GcLet)|= const_app c vl ~: T ->
     exists l, exists Us, exists v, exists vl',
-      vl = vl' ++ v :: nil /\ c = Const.matches l /\ length l = length vl' /\
-      exists K',
-        proper_instance (K & K') (Delta.type (Const.matches l)) Us /\
-        K & K'; empty |= v ~: nth 0 Us typ_def.
+      vl = rev (v :: vl') /\ c = Const.matches l /\ length l = length vl' /\
+      proper_instance K (Delta.type (Const.matches l)) Us /\
+      K; empty |(false,GcLet)|= v ~: nth 0 Us typ_def.
   Proof.
     intros.
     unfold const_app in H0.
-    destruct* (fold_app_inv' _ _ H0) as [K' [TL [TypC TypA]]]; clear H0.
+    use (fold_app_inv _ _ H0).
+    clear H0; destruct H1 as [TL [TypC TypA]].
     destruct c.
       elim (tag_is_const _ _ _ H TypC TypA).
     exists l.
-    destruct* (typing_cst_inv TypC) as [K'' [Us [Kok [PI E]]]]; clear TypC.
+    inversions TypC; try discriminate. clear TypC H5.
     exists Us.
     simpl in H.
-    unfold sch_open in E; simpl in E.
-    induction vl using rev_ind. discriminate. clear IHvl.
-    induction TL using rev_ind.
-      destruct vl; elim TypA.
-    clear IHTL.
-    exists x. exists vl.
-    assert (length l = length vl).
-      rewrite app_length in H. rewrite plus_comm in H. simpl in H.
-      inversion* H.
-    clear H; intuition.
-    assert (length vl = length TL).
-      generalize (For_all2_length _ _ _ TypA); intro.
-      repeat (rewrite app_length in H; rewrite plus_comm in H; simpl in H).
-      inversions* H.
-    destruct* (For_all2_app' _ _ _ _ _ TypA).
-    exists (K' & K''). rewrite <- concat_assoc.
-    split*.
-    simpl in H2. destruct H2 as [Typx _].
-    rewrite fold_right_app in E. simpl in E.
-    destruct (fold_arrow_eq _ _ _ _ _ (sym_equal E)); clear E.
-      simpl_list. rewrite* H0.
-    simpl in H2. inversions H2.
-    apply* typing_weaken_kinds'.
+    unfold sch_open in H1; simpl in H1.
+    rewrite <- (rev_involutive TL) in *.
+    destruct (rev TL) as [|T' TL'].
+      destruct vl. discriminate.
+      elim TypA.
+    rewrite <- (rev_involutive vl) in *.
+    destruct (rev vl) as [|v vl'].
+      discriminate.
+    exists v. exists vl'.
+    rewrite rev_length in H. simpl in H; inversion* H.
+    intuition.
+    use (For_all2_rev _ _ _ TypA); clear TypA.
+    autorewrite with list in H0.
+    simpl in H0; destruct H0 as [Typv TypA].
+    rewrite cons_append in H1.
+    rewrite distr_rev in H1.
+    rewrite fold_right_app in H1. simpl in H1.
+    destruct (fold_arrow_eq _ _ _ _ _ H1); clear H1.
+      autorewrite with list.
+      rewrite H3. apply* For_all2_length.
+    simpl in H0. inversions* H0.
   Qed.
 
   Lemma const_arity_ok : forall c vl K T,
     list_for_n value (S(Const.arity c)) vl ->
-    K ; empty |= const_app c vl ~: T ->
-    exists n, exists t1, exists t2, exists tl,
+    K ; empty |(false,GcLet)|= const_app c vl ~: T ->
+    exists n:nat, exists t1:trm, exists t2:trm, exists tl:list trm,
       Delta.rule n t1 t2 /\ list_for_n term n tl /\
       const_app c vl = trm_inst t1 tl.
   Proof.
     intros.
     destruct (const_arity_ok0 _ _ (proj1 H) H0) as
-      [l [Us [v [vl' [Evl [Ec [Hvl' [K' [PI Typv]]]]]]]]]; clear H0.
+      [l [Us [v [vl' [Evl [Ec [Hvl' [PI Typv]]]]]]]]; clear H0.
     subst.
     exists (S (length l)).
     destruct PI as [_ [_ WK]].
@@ -1294,7 +590,7 @@ Module SndHyp.
       inversion H0.
     destruct H as [_ Val].
     use (list_forall_rev Val); clear Val.
-    rewrite distr_rev in H. simpl in H.
+    rewrite rev_involutive in H.
     inversions H; clear H.
     destruct H3 as [vn Hv].
     use (proj1 WK). inversions H; clear H WK.
@@ -1303,30 +599,27 @@ Module SndHyp.
     clear vn Hv.
     subst.
     destruct (typing_tag_inv _ _ Typv) as
-      [t [T' [k [K'' [EQ [Typa [Bk Ek]]]]]]]; clear Typv.
-    forward (binds_concat_ok K'' H1) as Bk'.
-      apply (proj1 (proj1 (typing_regular Typa))).
-    use (binds_func Bk' Bk). inversion H; subst; clear H H1 Bk'.
+      [t [T' [k [EQ [Typa [Bk Ek]]]]]]; clear Typv.
+    use (binds_func H1 Bk). inversion H; subst; clear H H1.
     destruct H4 as [[_ High] _].
     destruct Ek as [[Low _] _].
     destruct k as [[kl kh] kr]; simpl in *.
     destruct* kh as [kh|].
-    use (proj2 (proj1 (typing_regular Typa)) _ _ Bk).
-    simpl in H.
-    unfold Cstr.valid in H. simpl in H.
-    use (subset_trans Low (subset_trans (proj1 (proj2 H)) High) (in_same l')).
-    clear H High Low kl kh kr Bk x Us.
-    use (mkset_in _ H0); clear H0.
+    use (proj2 (proj41 (typing_regular Typa)) _ _ Bk).
+    simpl in H. destruct H.
+    unfold Cstr.valid in H0. simpl in H0.
+    use (subset_trans Low (subset_trans (proj1 H0) High) (in_same l')).
+    clear H High Low kl kh kr Bk H0 x Us.
+    use (mkset_in _ H1); clear H1.
     destruct (exists_nth var_default _ _ H) as [n [Hlen EQ]].
     clear H; subst l'.
     exists (Delta.matches_lhs l n).
     exists (Delta.matches_rhs n).
-    exists (t :: vl').
+    exists (t :: rev vl').
     split3.
       unfold Delta.rule. exists l; exists n. auto.
-      split*. simpl. rewrite* Hvl'.
+      split*. simpl. rewrite rev_length. rewrite* Hvl'.
       constructor; auto.
-      rewrite <- rev_involutive.
       apply* list_forall_rev.
       apply (list_forall_imp _ value_regular H2).
     unfold Delta.matches_lhs.
@@ -1337,7 +630,8 @@ Module SndHyp.
     rewrite fold_left_app.
     simpl.
     rewrite Hvl'.
-    rewrite <- (map_inst_bvar t vl').
+    rewrite <- (rev_length vl').
+    rewrite <- (map_inst_bvar t (rev vl')).
     auto.
   Qed.
     
